Split off `SortedMap` into its own file

SplayTree4Lean/SplayMap.lean
@@ -272,7 +272,7 @@ def atRight (t : SplayMap α β) (x : α) : Prop :=
 
 -- TODO: do we use the three above functions anywhere? should we use them in `locationOf`?
 
-/--
+/-
 Looks for a value `x` in a `SplayMap`.
 If found, splays the tree at that node, executing zig-zig and zig-zag steps
 but *not* a zig step.
@@ -280,49 +280,50 @@ That is, if `x` ends up as a child of the root, a final rotation to bring it to
 the root is *not* performed.
 This is necessary for recursion to work in the `splay` function.
 -/
-def splayButOne (t : SplayMap α β) (x : α) : SplayMap α β :=
-  match t with
-  | nil => nil
-  | node yk yv yL yR =>
-      if x = yk then
-        t
-      else if x < yk then
-        let yL' := yL.splayButOne x
-        match yL'.locationOf x with
-        | Location.root => node yk yv yL' yR
-        | Location.left =>
-          match rotateLeftChild (node yk yv yL' yR) with
-          | some t1 =>
-            match rotateLeftChild t1 with
-            | some t2 => t2
-            | none => t1
-          | none => node yk yv yL' yR
-        | Location.right =>
-          match rotateRightChild yL' with
-          | some newYl =>
-            match rotateLeftChild (node yk yv newYl yR) with
-            | some t' => t'
-            | none => node yk yv newYl yR
-          | none => node yk yv yL' yR
-        | none => sorry
-      else
-        let yR' := yR.splayButOne x
-        match yR'.locationOf x with
-        | Location.root => node yk yv yL yR'
-        | Location.right =>
-          match rotateRightChild (node yk yv yL yR') with
-          | some t1 =>
-            match rotateRightChild t1 with
-            | some t2 => t2
-            | none => t1
-          | none => node yk yv yL yR'
-        | Location.left =>
-          match rotateLeftChild yR' with
-          | some newYr =>
-            match rotateRightChild (node yk yv yL newYr) with
-            | some t' => t'
-            | none => node yk yv yL newYr
-          | none => node yk yv yL yR'
+
+-- def splayButOne (t : SplayMap α β) (x : α) : SplayMap α β :=
+--   match t with
+--   | nil => nil
+--   | node yk yv yL yR =>
+--       if x = yk then
+--         t
+--       else if x < yk then
+--         let yL' := yL.splayButOne x
+--         match yL'.locationOf x with
+--         | Location.root => node yk yv yL' yR
+--         | Location.left =>
+--           match rotateLeftChild (node yk yv yL' yR) with
+--           | some t1 =>
+--             match rotateLeftChild t1 with
+--             | some t2 => t2
+--             | none => t1
+--           | none => node yk yv yL' yR
+--         | Location.right =>
+--           match rotateRightChild yL' with
+--           | some newYl =>
+--             match rotateLeftChild (node yk yv newYl yR) with
+--             | some t' => t'
+--             | none => node yk yv newYl yR
+--           | none => node yk yv yL' yR
+--         | none => sorry
+--       else
+--         let yR' := yR.splayButOne x
+--         match yR'.locationOf x with
+--         | Location.root => node yk yv yL yR'
+--         | Location.right =>
+--           match rotateRightChild (node yk yv yL yR') with
+--           | some t1 =>
+--             match rotateRightChild t1 with
+--             | some t2 => t2
+--             | none => t1
+--           | none => node yk yv yL yR'
+--         | Location.left =>
+--           match rotateLeftChild yR' with
+--           | some newYr =>
+--             match rotateRightChild (node yk yv yL newYr) with
+--             | some t' => t'
+--             | none => node yk yv yL newYr
+--          | none => node yk yv yL yR'
 
 -- theorem splayButOneMemberLocation (t : SplayMap α β) (x : α) (h : x ∈ t) :
 --     (t.splayButOne x).locationOf x ≠ .idk := by
@@ -349,28 +350,28 @@ def splayButOne (t : SplayMap α β) (x : α) : SplayMap α β :=
 Looks for a value `x` in a `SplayMap`.
 If found, splays the tree at that node.
 -/
-def splay (t : SplayMap α β) (x : α) (h : x ∈ t) : SplayMap α β :=
-  let t' := t.splayButOne x
-  let loc := t'.locationOf x
-  have h' : loc ≠ .idk := splayButOneMemberLocation t x h
-  match loc with
-  | .root => t
-  | .left => rotateLeftChild t
-  | .right => rotateRightChild t
-  | .idk => by trivial
+-- def splay (t : SplayMap α β) (x : α) (h : x ∈ t) : SplayMap α β :=
+--   let t' := t.splayButOne x
+--   let loc := t'.locationOf x
+--   have h' : loc ≠ .idk := splayButOneMemberLocation t x h
+--   match loc with
+--   | .root => t
+--   | .left => rotateLeftChild t
+--   | .right => rotateRightChild t
+--   | .idk => by trivial
 
-theorem splay_preserves_membership
-    (t : SplayMap α β) (x : α) (h : x ∈ t) : x ∈ splay t x h := by
-  let t' := t.splayButOne x
-  let loc := t'.locationOf x
-  have h' : loc ≠ .idk := splayButOneMemberLocation t x h
-  have mem_sbo : x ∈ t' := by sorry
-
-  match loc with
-  | .root => sorry
-  | .left => sorry
-  | .right => sorry
-  | .idk => simp at h'
+-- theorem splay_preserves_membership
+--     (t : SplayMap α β) (x : α) (h : x ∈ t) : x ∈ splay t x h := by
+--   let t' := t.splayButOne x
+--   let loc := t'.locationOf x
+--   have h' : loc ≠ .idk := splayButOneMemberLocation t x h
+--   have mem_sbo : x ∈ t' := by sorry
+--
+--   match loc with
+--   | .root => sorry
+--   | .left => sorry
+--   | .right => sorry
+--   | .idk => simp at h'
 
 
 -- theorem splayMember (t : SplayMap α β) (x : α) (h : x ∈ t) :
@@ -425,8 +426,8 @@ def get (t : SplayMap α β) (x : α) : SplayMap α β × Option β :=
   -- | none => (t, none) -- means t is nil
   -- | some yk => sorry
 
-/-- Doesn't work, needs rewriting `splay?`. -/
-def split (t : SplayMap α β) (x : α) (h : x ∈ t) : SplayMap α β × SplayMap α β :=
+/- Doesn't work, needs rewriting `splay?`. -/
+/- def split (t : SplayMap α β) (x : α) (h : x ∈ t) : SplayMap α β × SplayMap α β :=
   let t' := t.splay x h
   have h' : x ∈ t' := splay_preserves_membership t x h
   match t' with
@@ -434,278 +435,67 @@ def split (t : SplayMap α β) (x : α) (h : x ∈ t) : SplayMap α β × SplayM
   | node yk yv yL yR =>
       if x ≤ yk then (yL, node yk yv nil yR)
       else (node yk yv yL nil, yR)
+-/
 
-/-- Joins two splay trees where all keys in A are less than all keys in B -/
-def join (A B : SplayMap α β) : SplayMap α β :=
-  match A, B with
-  | nil, _ => B
-  | _, nil => A
-  | A, B =>
-      -- Find and splay the max element in A
-      let (maxK, maxV) := A.max (by sorry)
-      let A' := A.splay maxK (by sorry)
-      -- Now max element is at root of A'
-      match A' with
-      | node _ _ l _ => node maxK maxV l B
-      | nil => nil
+/- Joins two splay trees where all keys in A are less than all keys in B -/
+-- def join (A B : SplayMap α β) : SplayMap α β :=
+--   match A, B with
+--   | nil, _ => B
+--   | _, nil => A
+--   | A, B =>
+--       -- Find and splay the max element in A
+--       let (maxK, maxV) := A.max (by sorry)
+--       let A' := A.splay maxK (by sorry)
+--       -- Now max element is at root of A'
+--       match A' with
+--       | node _ _ l _ => node maxK maxV l B
+--       | nil => nil
 
-/-- Doesn't work, needs rewriting `splay?`. -/
-def insert (t : SplayMap α β) (xk : α) (xv : β) : SplayMap α β :=
-  match t.search? xk with
-  | none =>
-    let (L, R) := t.split xk (by sorry)
-    node xk xv L R
-  | some _ =>
-    let t' := t.splay xk (by sorry)
-    match t' with
-    | node _ _ l r => node xk xv l r
-    | nil => nil
+/- Doesn't work, needs rewriting `splay?`. -/
+-- def insert (t : SplayMap α β) (xk : α) (xv : β) : SplayMap α β :=
+--   match t.search? xk with
+--   | none =>
+--     let (L, R) := t.split xk (by sorry)
+--     node xk xv L R
+--   | some _ =>
+--     let t' := t.splay xk (by sorry)
+--     match t' with
+--     | node _ _ l r => node xk xv l r
+--     | nil => nil
 
 theorem max_mem (t : SplayMap α β) (h : t ≠ nil) :
-    (t.max h).1 ∈ t := by sorry
+    (t.max h) ∈ t := by sorry
 
-def delete (t : SplayMap α β) (x : α) (h : x ∈ t) : SplayMap α β :=
-  let t' := t.splay x h  -- First splay the node to delete to the root
-  have h' : x ∈ t' := splay_preserves_membership t x h
-  match t' with
-  | nil => absurd h' (noMemNil x)
-  | node k v l r =>
-    if x = k then
-      let (maxK, maxV) := l.max (by sorry)
-      let l' := l.splay maxK (by
-        simp [Membership.mem, splayMem]
-        apply l.max_mem (by sorry))
-      match l' with
-        | node _ _ ll lr => node maxK maxV ll r
-        | nil => nil
-      -- match l.max? with
-      -- | none => r
-      -- | some (maxK, maxV) =>
-      --     -- Splay the max of left subtree to root
-      --     let l' := l.splay maxK (by
-      --       simp [Membership.mem, splayMem]
-      --       exact l.max_mem (by sorry))
-      --     match l' with
-      --     | node _ _ ll lr => node maxK maxV ll r
-      --     | nil => nil
-    else
-      -- Prove contradiction
-      sorry
+-- def delete (t : SplayMap α β) (x : α) (h : x ∈ t) : SplayMap α β :=
+--   let t' := t.splay x h  -- First splay the node to delete to the root
+--   have h' : x ∈ t' := splay_preserves_membership t x h
+--   match t' with
+--   | nil => absurd h' (noMemNil x)
+--   | node k v l r =>
+--     if x = k then
+--       let (maxK, maxV) := l.max (by sorry)
+--       let l' := l.splay maxK (by
+--         simp [Membership.mem, splayMem]
+--         apply l.max_mem (by sorry))
+--       match l' with
+--         | node _ _ ll lr => node maxK maxV ll r
+--         | nil => nil
+--       -- match l.max? with
+--       -- | none => r
+--       -- | some (maxK, maxV) =>
+--       --     -- Splay the max of left subtree to root
+--       --     let l' := l.splay maxK (by
+--       --       simp [Membership.mem, splayMem]
+--       --       exact l.max_mem (by sorry))
+--       --     match l' with
+--       --     | node _ _ ll lr => node maxK maxV ll r
+--       --     | nil => nil
+--     else
+--       -- Prove contradiction
+--       sorry
 
-/-- Builds a `SplayMap` from a `List` by inserting its elements one-by-one. -/
-def fromList (L : List (α × β)) : SplayMap α β :=
-  L.foldl (fun t (xk, xv) => t.insert xk xv) nil
+/- Builds a `SplayMap` from a `List` by inserting its elements one-by-one. -/
+-- def fromList (L : List (α × β)) : SplayMap α β :=
+--   L.foldl (fun t (xk, xv) => t.insert xk xv) nil
 
 end SplayMap
-
-def SortedMap (α : Type u) (β : Type v) [LinearOrder α] :=
-  { t : SplayMap α β // SplayMap.is_sorted t }
-
-instance [DecidableEq (SplayMap α β)]: DecidableEq (SortedMap α β) :=
-  fun s t => if h : s.val = t.val then isTrue (Subtype.eq h) else isFalse (fun p => by cases p; contradiction)
-
-namespace SortedMap
-open SplayMap
-
-def nil : SortedMap α β :=
-  ⟨SplayMap.nil, trivial⟩
-
-omit [DecidableEq α] [DecidableEq β] in
-theorem sorted_nil_iff (t : SortedMap α β) : t = nil ↔ t.val = .nil := by
-  apply Iff.intro <;> intro h
-  · subst h
-    rfl
-  · apply Subtype.eq
-    assumption
-
-#eval 2 + 3
-
-omit [DecidableEq α] [DecidableEq β] in
-@[simp]
-theorem sorted_not_nil_implies (t : SortedMap α β) : t ≠ nil → t.val ≠ .nil := by
-  simp [sorted_nil_iff]
-
-def key (t : SortedMap α β) (h : t ≠ .nil) : α :=
-  t.val.key (by simp [h])
-
-def value (t : SortedMap α β) (h : t ≠ nil) : β :=
-  t.val.value (by simp [h])
-
-def left (t : SortedMap α β) (h : t ≠ nil) : SortedMap α β :=
-  ⟨t.val.left h', sorted_implies_left_sorted t.val h' t.prop⟩
-    where h' : t.val ≠ .nil := by simp [h]
-
-def right (t : SortedMap α β) (h : t ≠ nil) : SortedMap α β :=
-  ⟨t.val.right h', sorted_implies_right_sorted t.val h' t.prop⟩
-    where h' : t.val ≠ .nil := by simp [h]
-
-def max (t : SortedMap α β) (h : t ≠ nil) : α :=
-  have h0 : t.val ≠ SplayMap.nil := by simp [h]
-  if h' : t.right h = nil then
-    t.val.key h0
-  else
-    (t.right h).max h'
-termination_by t.val.size
-decreasing_by (exact size_mono_right t.val h0)
-
-def min (t : SortedMap α β) (h : t ≠ nil) : α :=
-  have h0 : t.val ≠ SplayMap.nil := by simp [h]
-  if h' : (t.left h) = nil then
-    t.val.key h0
-  else
-    (t.left h).min h'
-termination_by t.val.size
-decreasing_by (exact size_mono_left t.val h0)
-
-theorem plus_one (n : ℕ) : n + 1 > n := by
-  induction n with
-  | zero => trivial
-  | succ n => simp
-
-def rotateLeftChild (t : SortedMap α β) (h1 : t ≠ nil) (h2 : t.left h1 ≠ nil) : SortedMap α β :=
-  -- let t' := match t.val with
-  -- | node yk yv (node ylk ylv yLL yLR) yR =>
-  --   node ylk ylv yLL (node yk yv yLR yR) -- how is Lean so smart?!
-  -- | node yk yv .nil yR => sorry
-  -- | .nil => sorry
-  have ht : t.val ≠ .nil := by simp [h1]
-  have htl : t.val.left ht ≠ .nil := by sorry
-  let t' := SplayMap.rotateLeftChild t.val ht htl
-  have h' : (SplayMap.rotateLeftChild t.val ht htl).is_sorted := by
-    induction t.val with
-    | nil => 
-      have hh : t.val = .nil := by simp_all!
-      sorry
-    | node yk yv yL yR ihL ihR => sorry
-    match h : t.val with
-    | .nil =>
-      contradiction
-    | node yk yv .nil yR =>
-      have htl' : t.val.left ht = .nil := by simp_all! only
-      contradiction
-    | node yk yv (node ylk ylv yLL yLR) yR =>
-      simp_all [SplayMap.rotateLeftChild, t', ht]
-      match t.val, ht, htl with
-      | node yk yv (node ylk ylv yLL yLR) yR, h1, h2 =>
-        simp only
-      -- unfold SplayMap.is_sorted
-      match t' with
-      | .nil => trivial
-      | node _ _ l r => simp only
-      have hl : (t.1.left h).is_sorted := sorted_implies_left_sorted t.1 h t.2
-      have htl : t.1.left h = l := by
-        simp [ht]
-        rw [SplayMap.left]
-      have hl' : l.is_sorted := by simp_all
-      have hr : (t.1.right h).is_sorted := sorted_implies_right_sorted t.1 h t.2
-      have htr : t.1.right h = r := by
-        simp [ht]
-        rw [SplayMap.right]
-      have hr' : r.is_sorted := by simp_all
-
-      -- unfold SplayMap.is_sorted
-      -- match t' with
-      -- | .nil => trivial
-      -- | .node _ _ _ _ =>
-      -- exact h''
-  ⟨t', h'⟩
-
-def rotateRightChild (t : SortedMap α β) (h1 : t.val ≠ SplayMap.nil) (h2 : (t.val).right h1 ≠ SplayMap.nil) : SortedMap α β :=
-  let t' := (t.val).rotateRightChild h1 h2
-  have h' : t'.is_sorted := by sorry
-  ⟨t', h'⟩
-
-/--
-Looks for a value `x` in a `SplayMap`.
-If found, splays the tree at that node, executing zig-zig and zig-zag steps
-but *not* a zig step.
-That is, if `x` ends up as a child of the root, a final rotation to bring it to
-the root is *not* performed.
-This is necessary for recursion to work in the `splay` function.
--/
-def splayButOne (t : SortedMap α β) (x : α) : SortedMap α β :=
-  match t.val with
-  | .nil => nil
-  | .node yk yv yL yR =>
-      if x = yk then
-        t
-      else if x < yk then
-        let yL' := yL.splayButOne x
-        match yL'.locationOf x with
-        | Location.root => ⟨.node yk yv yL' yR, sorry⟩
-        | Location.left =>
-          match (node yk yv yL' yR).rotateLeftChild (sorry) with
-          | t1 =>
-            match rotateLeftChild t1 with
-            | some t2 => t2
-            | none => t1
-          | none => node yk yv yL' yR
-        | Location.right =>
-          match rotateRightChild yL' with
-          | some newYl =>
-            match rotateLeftChild (node yk yv newYl yR) with
-            | some t' => t'
-            | none => node yk yv newYl yR
-          | none => node yk yv yL' yR
-        | none => sorry
-      else
-        let yR' := yR.splayButOne x
-        match yR'.locationOf x with
-        | Location.root => node yk yv yL yR'
-        | Location.right =>
-          match rotateRightChild (node yk yv yL yR') with
-          | some t1 =>
-            match rotateRightChild t1 with
-            | some t2 => t2
-            | none => t1
-          | none => node yk yv yL yR'
-        | Location.left =>
-          match rotateLeftChild yR' with
-          | some newYr =>
-            match rotateRightChild (node yk yv yL newYr) with
-            | some t' => t'
-            | none => node yk yv yL newYr
-          | none => node yk yv yL yR'
-
--- theorem splayButOneMemberLocation (t : SplayMap α β) (x : α) (h : x ∈ t) :
---     (t.splayButOne x).locationOf x ≠ .idk := by
---   cases t with
---   | nil =>
---       absurd h
---       exact noMemNil x
---   | node yk yv yL yR =>
---       if h₁ : x = yk then
---         subst h₁
---         have h' : (node x yv yL yR).locationOf x = .root := by
---           simp_all!
---         intro h''
---         have p : Location.root ≠ Location.idk := by
---           intro q
---           trivial
---         simp_all!
---       else if x < yk then
---         sorry
---       else
---         sorry
-
-/-
-Looks for a value `x` in a `SplayMap`.
-If found, splays the tree at that node.
--/
-def splay (t : SplayMap α β) (x : α) (h : x ∈ t) : SplayMap α β :=
-  let t' := t.splayButOne x
-  let loc := t'.locationOf x
-  have h' : loc ≠ .idk := splayButOneMemberLocation t x h
-  match loc with
-  | .root => t
-  | .left => rotateLeftChild t
-  | .right => rotateRightChild t
-  | .idk => by trivial
-
-end SortedMap
-
-def five? : Option Nat := Option.some 5
-#check five?
-
-#eval five?.get!
-#eval (2, 3).1
